Irrelevance conquered!

theories/LogicalRelation/Irrelevance.v
@@ -1,6 +1,7 @@
 (** * LogRel.LogicalRelation.Irrelevance: symmetry and irrelevance of the logical relation. *)
+Require Import PeanoNat.
 From LogRel.AutoSubst Require Import core unscoped Ast Extra.
-From LogRel Require Import Notations Utils BasicAst Context NormalForms Weakening GenericTyping LogicalRelation DeclarativeInstance.
+From LogRel Require Import Notations Utils BasicAst LContexts Context NormalForms Weakening GenericTyping LogicalRelation DeclarativeInstance.
 From LogRel.LogicalRelation Require Import Induction ShapeView Reflexivity.
 
 Set Universe Polymorphism.
@@ -25,14 +26,14 @@ Section EquivLRPack.
 
   Notation "A <≈> B" := (prod@{v v} (A -> B) (B -> A)) (at level 90).
 
-  Definition equivLRPack {Γ Γ' A A'} (P: LRPack@{i} Γ A) (P': LRPack@{i'} Γ' A'):=
+  Definition equivLRPack {wl wl' Γ Γ' A A'} (P: LRPack@{i} wl Γ A) (P': LRPack@{i'} wl' Γ' A'):=
     and3@{v v v} 
-      (forall B, [P | Γ ||- A ≅ B] <≈> [P' | Γ' ||- A' ≅ B])
-      (forall t, [P | Γ ||- t : A] <≈> [P' | Γ' ||- t : A'])
-      (forall t u, [P | Γ ||- t ≅ u : A] <≈> [P' | Γ' ||- t ≅ u : A']).
+      (forall B, [P | Γ ||- A ≅ B]< wl > <≈> [P' | Γ' ||- A' ≅ B]< wl' >)
+      (forall t, [P | Γ ||- t : A]< wl > <≈> [P' | Γ' ||- t : A']< wl' >)
+      (forall t u, [P | Γ ||- t ≅ u : A]< wl > <≈> [P' | Γ' ||- t ≅ u : A']< wl' >).
 End EquivLRPack.
 
-Lemma symLRPack@{i i' v} {Γ Γ' A A'} {P: LRPack@{i} Γ A} {P': LRPack@{i'} Γ' A'} :
+Lemma symLRPack@{i i' v} {wl wl' Γ Γ' A A'} {P: LRPack@{i} wl Γ A} {P': LRPack@{i'} wl' Γ' A'} :
     equivLRPack@{i i' v} P P' -> equivLRPack@{i' i v} P' P.
 Proof.
   intros [eqT rTm eqTm]; constructor;split ;
@@ -49,127 +50,293 @@ avoid having to basically duplicate their proofs. *)
 
 Section ΠIrrelevanceLemmas.
 Universe i j k l i' j' k' l' v.
-Context {Γ lA A lA' A'} 
-  (ΠA : PiRedTyPack@{i j k l} Γ A lA) 
-  (ΠA' : PiRedTyPack@{i' j' k' l'} Γ A' lA')
+Context {wl Γ lA A lA' A'} 
+  (ΠA : PiRedTyPack@{i j k l} wl Γ A lA) 
+  (ΠA' : PiRedTyPack@{i' j' k' l'} wl Γ A' lA')
   (RA := LRPi' ΠA)
   (RA' := LRPi' ΠA')
-  (domRed := (@PiRedTyPack.domRed _ _ _ _ _ _ _ _ _ _ _ _ _ _ _ _ ΠA))
-  (domRed' := (@PiRedTyPack.domRed _ _ _ _ _ _ _ _ _ _ _ _ _ _ _ _ ΠA'))
-  (codRed := (@PiRedTyPack.codRed  _ _ _ _ _ _ _ _ _ _ _ _ _ _ _ _ ΠA))
-  (codRed' := (@PiRedTyPack.codRed  _ _ _ _ _ _ _ _ _ _ _ _ _ _ _ _ ΠA'))
-  (eqPi : [Γ |- PiRedTyPack.prod ΠA ≅ PiRedTyPack.prod ΠA']).
+  (domN := @PiRedTyPack.domN _ _ _ _ _ _ _ _ _ _ _ _ _ _ _ _ _ ΠA)
+  (domN' := @PiRedTyPack.domN _ _ _ _ _ _ _ _ _ _ _ _ _ _ _ _ _ ΠA')
+  (domRed := (@PiRedTyPack.domRed _ _ _ _ _ _ _ _ _ _ _ _ _ _ _ _ _ ΠA))
+  (domRed' := (@PiRedTyPack.domRed _ _ _ _ _ _ _ _ _ _ _ _ _ _ _ _ _ ΠA'))
+  (codomN := @PiRedTyPack.codomN _ _ _ _ _ _ _ _ _ _ _ _ _ _ _ _ _ ΠA)
+  (codomN' := @PiRedTyPack.codomN _ _ _ _ _ _ _ _ _ _ _ _ _ _ _ _ _ ΠA')
+  (codRed := (@PiRedTyPack.codRed _ _ _ _ _ _ _ _ _ _ _ _ _ _ _ _ _ ΠA))
+  (codRed' := (@PiRedTyPack.codRed  _ _ _ _ _ _ _ _ _ _ _ _ _ _ _ _ _ ΠA'))
+  (eqPi : [Γ |- PiRedTyPack.prod ΠA ≅ PiRedTyPack.prod ΠA']< wl >).
 
-Context (eqvDom : forall {Δ} (ρ : Δ ≤ Γ) (wfΔ : [  |- Δ]),
-          equivLRPack@{k k' v} (domRed Δ ρ wfΔ) (domRed' Δ ρ wfΔ))
-        (eqvCod : forall {Δ a} (ρ : Δ ≤ Γ) (wfΔ : [  |- Δ])
-          (ha : [domRed Δ ρ wfΔ| Δ ||- a : _])
-          (ha' : [domRed' Δ ρ wfΔ | Δ ||- a : _]),
-          equivLRPack@{k k' v} (codRed Δ a ρ wfΔ ha) (codRed' Δ a ρ wfΔ ha')).
+Context
+  (eqvDomN : nat)
+  (eqvDom : forall {Δ wl'} (ρ : Δ ≤ Γ) (τ : wl' ≤ε wl)
+                   (Ninfl : domN <= length wl')
+                   (Ninfl' : domN' <= length wl')
+                   (Ninfl'' : eqvDomN <= length wl')
+                   (wfΔ : [  |- Δ]< wl' >),
+      equivLRPack@{k k' v} (domRed Δ wl' ρ τ Ninfl wfΔ)
+        (domRed' Δ wl' ρ τ Ninfl' wfΔ))
+  (eqvCodN : forall {Δ a wl'} (ρ : Δ ≤ Γ) (τ : wl' ≤ε wl)
+                   (Ninfl : domN <= length wl')
+                   (Ninfl' : domN' <= length wl')
+                   (Ninfl'' : eqvDomN <= length wl')
+                   (wfΔ : [  |- Δ]< wl' >)
+          (ha : [domRed Δ wl' ρ τ Ninfl wfΔ| Δ ||- a : _]< wl' >)
+          (ha' : [domRed' Δ wl' ρ τ Ninfl' wfΔ | Δ ||- a : _]< wl' >),
+      nat)
+   (eqvCod : forall {Δ a wl'} (ρ : Δ ≤ Γ) (τ : wl' ≤ε wl)
+                    (Ninfl : domN <= length wl')
+                    (Ninfl' : domN' <= length wl')
+                    (Ninfl'' : eqvDomN <= length wl')
+                    (wfΔ : [  |- Δ]< wl' >)
+                    (ha : [domRed Δ wl' ρ τ Ninfl wfΔ| Δ ||- a : _]< wl' >)
+                    (ha' : [domRed' Δ wl' ρ τ Ninfl' wfΔ | Δ ||- a : _]< wl' >)
+                    {wl''} (τ' : wl'' ≤ε wl')
+                    (Minfl : codomN _ _ _ ρ τ Ninfl wfΔ ha <= length wl'')
+                    (Minfl' : codomN' _ _ _ ρ τ Ninfl' wfΔ ha' <= length wl'')
+                    (Minfl'' : eqvCodN ρ τ Ninfl Ninfl' Ninfl'' wfΔ ha ha' <= length wl''),
+       equivLRPack@{k k' v} (codRed Δ a wl' ρ τ Ninfl wfΔ ha wl'' τ' Minfl)
+              (codRed' Δ a wl' ρ τ Ninfl' wfΔ ha' wl'' τ' Minfl')).
 
-Lemma ΠIrrelevanceTyEq B : [Γ ||-<lA> A ≅ B | RA] -> [Γ ||-<lA'> A' ≅ B | RA'].
+Lemma ΠIrrelevanceTyEq B :
+  [Γ ||-<lA> A ≅ B | RA]< wl > -> [Γ ||-<lA'> A' ≅ B | RA']< wl >.
 Proof.
-  intros [] ; cbn in *; econstructor.
-  - now gen_typing.
+  intros [] ; cbn in *.
+  unshelve econstructor ; [exact dom | exact cod | ..].
+  - exact (max (max domN0 domN) eqvDomN).
+  - intros ; cbn in *.
+    unshelve eapply (max (max _ _) _).
+    + unshelve eapply (codomN Δ a l' ρ τ _ h).
+      eapply Nat.max_lub_r.
+      now eapply Nat.max_lub_l.
+      unshelve eapply eqvDom ; try assumption.
+      now eapply Nat.max_lub_r.
+    + unshelve eapply (codomN0 Δ a l' ρ τ _ _) ; try assumption.
+      * eapply Nat.max_lub_r.
+        now eapply Nat.max_lub_l.
+      * eapply Nat.max_lub_l.
+        now eapply Nat.max_lub_l.
+      * unshelve  eapply eqvDom ; try assumption.
+        now eapply Nat.max_lub_r.
+    + unshelve eapply (eqvCodN Δ a l' ρ τ _ _ _) ; try assumption.
+      * eapply Nat.max_lub_r.
+        now eapply Nat.max_lub_l.
+      * now eapply Nat.max_lub_r.
+      * unshelve eapply eqvDom ; try assumption.
+        now eapply Nat.max_lub_r.
+  - assumption.
   - cbn; etransitivity; [|tea]; now symmetry.
-  - intros ; now apply eqvDom.
-  - intros; cbn; unshelve eapply eqvCod.
-    2: eauto.
-    now eapply eqvDom.
+  - intros.
+    unshelve eapply eqvDom ; try eapply PeanoNat.Nat.max_lub_r ; try now eapply PeanoNat.Nat.max_lub_l.
+    eassumption.
+    unshelve eapply domRed0.
+    eapply Nat.max_lub_l.
+    now eapply Nat.max_lub_l.
+  - intros; cbn in *.
+    unshelve eapply eqvCod ; cbn in *.
+    + eapply Nat.max_lub_r.
+      now eapply Nat.max_lub_l.
+    + now eapply Nat.max_lub_r.
+    + cbn in *.
+      unshelve eapply eqvDom ; try assumption.
+      now eapply Nat.max_lub_r.
+    + cbn in *.
+      eapply Nat.max_lub_l.
+      now eapply Nat.max_lub_l.
+    + cbn in *.
+      now eapply Nat.max_lub_r.
+    + unshelve eapply codRed0.
+      * eapply Nat.max_lub_l.
+        now eapply Nat.max_lub_l.
+      * eapply Nat.max_lub_r.
+        now eapply Nat.max_lub_l.
 Qed.
 
-Lemma ΠIrrelevanceTm t : [Γ ||-<lA> t : A | RA] -> [Γ ||-<lA'> t : A' | RA'].
+Lemma ΠIrrelevanceTm t : [Γ ||-<lA> t : A | RA]< wl > -> [Γ ||-<lA'> t : A' | RA']< wl >.
 Proof.
-  intros []; cbn in *; econstructor; tea.
+  intros []; cbn in *.
+  unshelve econstructor; [ tea | ..] ; cbn in *.
+  - refine (max (max redN domN) eqvDomN).
+  - intros.
+    unshelve refine (max (max _ _) _).
+    + unshelve refine (appN Δ a l' ρ τ _ _ _ _) ; try assumption. 
+      * eapply Nat.max_lub_r.
+        now eapply Nat.max_lub_l.
+      * eapply Nat.max_lub_l.
+        now eapply Nat.max_lub_l.
+      * unshelve eapply eqvDom ; try assumption.
+        now eapply Nat.max_lub_r.
+    + unshelve refine (codomN Δ a l' ρ τ _ _ _) ; try assumption. 
+      * eapply Nat.max_lub_r.
+        now eapply Nat.max_lub_l.
+      * unshelve eapply eqvDom ; try assumption.
+        now eapply Nat.max_lub_r.
+    + unshelve eapply (eqvCodN Δ a l' ρ τ _ _ _) ; try assumption.
+      * eapply Nat.max_lub_r.
+        now eapply Nat.max_lub_l.
+      * now eapply Nat.max_lub_r.
+      * unshelve eapply eqvDom ; try assumption.
+        now eapply Nat.max_lub_r.
   - now eapply redtmwf_conv.
+  - assumption.
   - apply (tm_nf_conv isnf).
-    + destruct ΠA'; simpl in *; now apply wft_prod.
-    + apply eqPi.
+    + destruct ΠA'; simpl in * ; apply eqPi.
   - now eapply convtm_conv.
   - intros; unshelve eapply eqvCod.
-    2: now auto.
-    now apply eqvDom.
+    + eapply Nat.max_lub_r.
+      now eapply Nat.max_lub_l.
+    + now eapply Nat.max_lub_r.
+    + cbn in *.
+      unshelve eapply eqvDom ; try assumption.
+      now eapply Nat.max_lub_r.
+    + eapply Nat.max_lub_r.
+      now eapply Nat.max_lub_l.
+    + now eapply Nat.max_lub_r.
+    + cbn in *.
+      eapply app.
+      eapply Nat.max_lub_l.
+      now eapply Nat.max_lub_l.
   - intros; unshelve eapply eqvCod, eq.
-    all: now eapply eqvDom.
+    all: try eapply eqvDom ; try eassumption.
+    all: try (eapply Nat.max_lub_r ;
+              now eapply Nat.max_lub_l).
+    all: try (eapply Nat.max_lub_l ;
+              now eapply Nat.max_lub_l).
+    all: try now eapply Nat.max_lub_r.
 Defined.
 
-Lemma ΠIrrelevanceTmEq t u : [Γ ||-<lA> t ≅ u : A | RA] -> [Γ ||-<lA'> t ≅ u : A' | RA'].
+Lemma ΠIrrelevanceTmEq t u : [Γ ||-<lA> t ≅ u : A | RA]< wl > -> [Γ ||-<lA'> t ≅ u : A' | RA']< wl >.
 Proof.
   intros [] ; cbn in *; unshelve econstructor.
   1,2: now eapply ΠIrrelevanceTm.
+  - exact (max (max eqN domN) eqvDomN).
+  - intros.
+    unshelve refine (max (max _ _) _).
+    + unshelve refine (eqappN Δ a l' ρ τ _ _ _ _) ; try assumption.
+      * eapply Nat.max_lub_r ; now eapply Nat.max_lub_l.
+      * eapply Nat.max_lub_l ; now eapply Nat.max_lub_l.
+      * unshelve eapply eqvDom ; try assumption.
+        now eapply Nat.max_lub_r.
+    + unshelve refine (codomN Δ a l' ρ τ _ _ _) ; try assumption. 
+      * eapply Nat.max_lub_r ; now eapply Nat.max_lub_l.
+      * unshelve eapply eqvDom ; try assumption.
+        now eapply Nat.max_lub_r.
+    + unshelve eapply (eqvCodN Δ a l' ρ τ _ _ _) ; try assumption.
+      * eapply Nat.max_lub_r.
+        now eapply Nat.max_lub_l.
+      * now eapply Nat.max_lub_r.
+      * unshelve eapply eqvDom ; try assumption.
+        now eapply Nat.max_lub_r.
   - now eapply convtm_conv.
   - intros; unshelve eapply eqvCod.
-    2: now auto.
-    now apply eqvDom.
+    + eapply Nat.max_lub_r ; now eapply Nat.max_lub_l.
+    + now eapply Nat.max_lub_r.
+    + cbn in *.
+      unshelve eapply eqvDom ; try assumption.
+      now eapply Nat.max_lub_r.
+    + eapply Nat.max_lub_r ; now eapply Nat.max_lub_l.
+    + now eapply Nat.max_lub_r.
+    + cbn in *.
+      eapply eqApp.
+      eapply Nat.max_lub_l ; now eapply Nat.max_lub_l.
 Qed.
 
 End ΠIrrelevanceLemmas.
 
 Lemma ΠIrrelevanceLRPack@{i j k l i' j' k' l' v}
-  {Γ lA A lA' A'} 
-  (ΠA : PiRedTyPack@{i j k l} Γ A lA) 
-  (ΠA' : PiRedTyPack@{i' j' k' l'} Γ A' lA')
+  {wl Γ lA A lA' A'} 
+  (ΠA : PiRedTyPack@{i j k l} wl Γ A lA) 
+  (ΠA' : PiRedTyPack@{i' j' k' l'} wl Γ A' lA')
   (RA := LRPi' ΠA)
   (RA' := LRPi' ΠA')
-  (domRed := (@PiRedTyPack.domRed _ _ _ _ _ _ _ _ _ _ _ _ _ _ _ _ ΠA))
-  (domRed' := (@PiRedTyPack.domRed _ _ _ _ _ _ _ _ _ _ _ _ _ _ _ _ ΠA'))
-  (codRed := (@PiRedTyPack.codRed  _ _ _ _ _ _ _ _ _ _ _ _ _ _ _ _ ΠA))
-  (codRed' := (@PiRedTyPack.codRed  _ _ _ _ _ _ _ _ _ _ _ _ _ _ _ _ ΠA'))
-  (eqPi : [Γ |- PiRedTyPack.prod ΠA ≅ PiRedTyPack.prod ΠA'])
-  (eqvDom : forall {Δ} (ρ : Δ ≤ Γ) (wfΔ : [  |- Δ]),
-          equivLRPack@{k k' v} (domRed Δ ρ wfΔ) (domRed' Δ ρ wfΔ))
-  (eqvCod : forall {Δ a} (ρ : Δ ≤ Γ) (wfΔ : [  |- Δ])
-          (ha : [Δ ||-<lA> a : _| domRed Δ ρ wfΔ])
-          (ha' : [Δ ||-<lA'> a : _| domRed' Δ ρ wfΔ ]),
-          equivLRPack@{k k' v} (codRed Δ a ρ wfΔ ha) (codRed' Δ a ρ wfΔ ha'))
-  : equivLRPack@{k k' v} RA RA'.
+  (domN := @PiRedTyPack.domN _ _ _ _ _ _ _ _ _ _ _ _ _ _ _ _ _ ΠA)
+  (domN' := @PiRedTyPack.domN _ _ _ _ _ _ _ _ _ _ _ _ _ _ _ _ _ ΠA')
+  (domRed := (@PiRedTyPack.domRed _ _ _ _ _ _ _ _ _ _ _ _ _ _ _ _ _ ΠA))
+  (domRed' := (@PiRedTyPack.domRed _ _ _ _ _ _ _ _ _ _ _ _ _ _ _ _ _ ΠA'))
+  (codomN := @PiRedTyPack.codomN _ _ _ _ _ _ _ _ _ _ _ _ _ _ _ _ _ ΠA)
+  (codomN' := @PiRedTyPack.codomN _ _ _ _ _ _ _ _ _ _ _ _ _ _ _ _ _ ΠA')
+  (codRed := (@PiRedTyPack.codRed  _ _ _ _ _ _ _ _ _ _ _ _ _ _ _ _ _ ΠA))
+  (codRed' := (@PiRedTyPack.codRed  _ _ _ _ _ _ _ _ _ _ _ _ _ _ _ _ _ ΠA'))
+  (eqPi : [Γ |- PiRedTyPack.prod ΠA ≅ PiRedTyPack.prod ΠA']< wl >)
+  (eqvDomN : nat)
+  (eqvDom : forall {Δ wl'} (ρ : Δ ≤ Γ) (τ : wl' ≤ε wl)
+                   (Ninfl : domN <= length wl')
+                   (Ninfl' : domN' <= length wl')
+                   (Ninfl'' : eqvDomN <= length wl')
+                   (wfΔ : [  |- Δ]< wl' >),
+      equivLRPack@{k k' v} (domRed Δ wl' ρ τ Ninfl wfΔ)
+        (domRed' Δ wl' ρ τ Ninfl' wfΔ))
+  (eqvCodN : forall {Δ a wl'} (ρ : Δ ≤ Γ) (τ : wl' ≤ε wl)
+                   (Ninfl : domN <= length wl')
+                   (Ninfl' : domN' <= length wl')
+                   (Ninfl'' : eqvDomN <= length wl')
+                   (wfΔ : [  |- Δ]< wl' >)
+          (ha : [domRed Δ wl' ρ τ Ninfl wfΔ| Δ ||- a : _]< wl' >)
+          (ha' : [domRed' Δ wl' ρ τ Ninfl' wfΔ | Δ ||- a : _]< wl' >),
+      nat)
+   (eqvCod : forall {Δ a wl'} (ρ : Δ ≤ Γ) (τ : wl' ≤ε wl)
+                    (Ninfl : domN <= length wl')
+                    (Ninfl' : domN' <= length wl')
+                    (Ninfl'' : eqvDomN <= length wl')
+                    (wfΔ : [  |- Δ]< wl' >)
+                    (ha : [domRed Δ wl' ρ τ Ninfl wfΔ| Δ ||- a : _]< wl' >)
+                    (ha' : [domRed' Δ wl' ρ τ Ninfl' wfΔ | Δ ||- a : _]< wl' >)
+                    {wl''} (τ' : wl'' ≤ε wl')
+                    (Minfl : codomN _ _ _ ρ τ Ninfl wfΔ ha <= length wl'')
+                    (Minfl' : codomN' _ _ _ ρ τ Ninfl' wfΔ ha' <= length wl'')
+                    (Minfl'' : eqvCodN ρ τ Ninfl Ninfl' Ninfl'' wfΔ ha ha' <= length wl''),
+       equivLRPack@{k k' v} (codRed Δ a wl' ρ τ Ninfl wfΔ ha wl'' τ' Minfl)
+         (codRed' Δ a wl' ρ τ Ninfl' wfΔ ha' wl'' τ' Minfl'))
+   : equivLRPack@{k k' v} RA RA'.
 Proof.
-  pose proof (eqvDom' := fun Δ ρ wfΔ => symLRPack (@eqvDom Δ ρ wfΔ)).
-  pose proof (eqvCod' := fun Δ a ρ wfΔ ha ha' => symLRPack (@eqvCod Δ a ρ wfΔ ha ha')).
+  pose proof (eqvDom' := fun Δ wl' ρ τ Ninfl Ninfl' Ninfl'' wfΔ =>
+                           symLRPack (@eqvDom Δ wl' ρ τ Ninfl Ninfl' Ninfl'' wfΔ)).
+  pose (eqvCodN' := fun Δ a wl' ρ τ Ninfl Ninfl' Ninfl'' wfΔ ha ha' =>
+                           @eqvCodN Δ a wl' ρ τ Ninfl' Ninfl Ninfl'' wfΔ ha' ha ).
+  pose proof (eqvCod' := fun Δ a wl' ρ τ Ninfl Ninfl' Ninfl'' wfΔ ha ha' wl'' τ' Minfl Minfl' Minfl'' =>
+                           symLRPack (@eqvCod Δ a wl' ρ τ Ninfl Ninfl' Ninfl'' wfΔ ha ha' wl'' τ' Minfl Minfl' Minfl'')).
   constructor.
-  - split; now apply ΠIrrelevanceTyEq.
-  - split; now apply ΠIrrelevanceTm.
-  - split; now apply ΠIrrelevanceTmEq.
+  - split ; unshelve eapply ΠIrrelevanceTyEq ; easy.
+  - split; unshelve eapply ΠIrrelevanceTm ; easy.
+  - split; unshelve eapply ΠIrrelevanceTmEq ; easy.
 Qed.
 
 (** *** Irrelevance for neutral types *)
 
 Lemma NeIrrelevanceLRPack@{i j k l i' j' k' l' v}
-  {Γ A A'} lA lA'
-  (neA : [Γ ||-ne A])
-  (neA' : [Γ ||-ne A'])
+  {wl Γ A A'} lA lA'
+  (neA : [Γ ||-ne A]< wl >)
+  (neA' : [Γ ||-ne A']< wl >)
   (RA := LRne_@{i j k l} lA neA)
   (RA' := LRne_@{i' j' k' l'} lA' neA')
-  (eqAA' : [Γ ||-ne A ≅ A' | neA ])
+  (eqAA' : [Γ ||-ne A ≅ A' | neA ]< wl >)
   : equivLRPack@{k k' v} RA RA'.
 Proof.
   destruct neA as [ty], neA' as [ty'], eqAA' as [ty0']; cbn in *.
   assert (ty0' = ty'); [|subst].
   { eapply redtywf_det; tea; constructor; now eapply ty_ne_whne. }
-  assert [Γ |- ty ≅ ty'] as convty by gen_typing.
+  assert [Γ |- ty ≅ ty']< wl > as convty by gen_typing.
   split.
   + intros ?; split; intros []; econstructor; cbn in *; tea.
     all: etransitivity ; [| tea]; tea; now symmetry.
   + intros ?; split; intros []; econstructor; cbn in *; tea.
     1,4: now eapply redtmwf_conv.
-    all: try match goal with |- Ne[ _ |- _ : _] => destruct red, red1; now eapply tm_ne_conv; first [eassumption|symmetry; eassumption|gen_typing] end.
+    all: try match goal with |- Ne[ _ |- _ : _]< _ > => destruct red, red1; now eapply tm_ne_conv; first [eassumption|symmetry; eassumption|gen_typing] end.
     all: now eapply convneu_conv.
   + intros ??; split; intros []; econstructor; cbn in *.
     1-2,6-7: now eapply redtmwf_conv.
     all: tea.
-    all: try match goal with |- Ne[ _ |- _ : _] => destruct red, red1; now eapply tm_ne_conv; first [eassumption|symmetry; eassumption|gen_typing] end.
+    all: try match goal with |- Ne[ _ |- _ : _]< _ > => destruct red, red1; now eapply tm_ne_conv; first [eassumption|symmetry; eassumption|gen_typing] end.
     all: now eapply convneu_conv.
 Qed.
 
 (** *** Lemmas for conversion of reducible neutral terms at arbitrary types *)
 
-Lemma NeNfconv {Γ k A A'} : [Γ |- A'] -> [Γ |- A ≅ A'] -> [Γ ||-NeNf k : A] -> [Γ ||-NeNf k : A'].
+Lemma NeNfconv {wl Γ k A A'} : [Γ |- A']< wl > -> [Γ |- A ≅ A']< wl > -> [Γ ||-NeNf k : A]< wl > -> [Γ ||-NeNf k : A']< wl >.
 Proof.
   intros ?? []; econstructor; tea. 2,3: gen_typing.
   now eapply tm_ne_conv.
 Qed.
 
-Lemma NeNfEqconv {Γ k k' A A'} : [Γ |- A'] -> [Γ |- A ≅ A'] -> [Γ ||-NeNf k ≅ k' : A] -> [Γ ||-NeNf k ≅ k' : A'].
+Lemma NeNfEqconv {wl Γ k k' A A'} : [Γ |- A']< wl > -> [Γ |- A ≅ A']< wl > -> [Γ ||-NeNf k ≅ k' : A]< wl > -> [Γ ||-NeNf k ≅ k' : A']< wl >.
 Proof.
   intros ?? []; econstructor; tea. 3: gen_typing.
   all: now eapply tm_ne_conv.
@@ -179,23 +346,23 @@ Qed.
 Section NatIrrelevant.
   Universe i j k l i' j' k' l'.
 
-  Context {Γ lA lA' A A'} (NA : [Γ ||-Nat A]) (NA' : [Γ ||-Nat A'])
+  Context {wl Γ lA lA' A A'} (NA : [Γ ||-Nat A]< wl >) (NA' : [Γ ||-Nat A']< wl >)
     (RA := LRNat_@{i j k l} lA NA) (RA' := LRNat_@{i' j' k' l'} lA' NA').
   
-  Lemma NatIrrelevanceTyEq B : [Γ ||-<lA> A ≅ B | RA] -> [Γ ||-<lA'> A' ≅ B | RA'].
+  Lemma NatIrrelevanceTyEq B : [Γ ||-<lA> A ≅ B | RA]< wl > -> [Γ ||-<lA'> A' ≅ B | RA']< wl >.
   Proof.
     intros []; now econstructor.
   Qed.
 
   Lemma NatIrrelevanceTm :
-    (forall t, [Γ ||-<lA> t : A | RA] -> [Γ ||-<lA'> t : A' | RA'])
+    (forall t, [Γ ||-<lA> t : A | RA]< wl > -> [Γ ||-<lA'> t : A' | RA']< wl >)
     × (forall t, NatProp NA t -> NatProp NA' t).
   Proof.
     apply NatRedInduction; now econstructor.
   Qed.
    
   Lemma NatIrrelevanceTmEq :
-    (forall t u, [Γ ||-<lA> t ≅ u : A | RA] -> [Γ ||-<lA'> t ≅ u : A' | RA'])
+    (forall t u, [Γ ||-<lA> t ≅ u : A | RA]< wl > -> [Γ ||-<lA'> t ≅ u : A' | RA']< wl >)
     × (forall t u, NatPropEq NA t u -> NatPropEq NA' t u).
   Proof.
     apply NatRedEqInduction; now econstructor.
@@ -203,7 +370,7 @@ Section NatIrrelevant.
 End NatIrrelevant.
 
 Lemma NatIrrelevanceLRPack@{i j k l i' j' k' l' v}
-  {Γ lA lA' A A'} (NA : [Γ ||-Nat A]) (NA' : [Γ ||-Nat A'])
+  {wl Γ lA lA' A A'} (NA : [Γ ||-Nat A]< wl >) (NA' : [Γ ||-Nat A']< wl >)
   (RA := LRNat_@{i j k l} lA NA) (RA' := LRNat_@{i' j' k' l'} lA' NA') :
   equivLRPack@{k k' v} RA RA'.
 Proof.
@@ -213,32 +380,72 @@ Proof.
   - split; apply NatIrrelevanceTmEq.
 Qed.
 
+Section BoolIrrelevant.
+  Universe i j k l i' j' k' l'.
+
+  Context {wl Γ lA lA' A A'} (NA : [Γ ||-Bool A]< wl >) (NA' : [Γ ||-Bool A']< wl >)
+    (RA := LRBool_@{i j k l} lA NA) (RA' := LRBool_@{i' j' k' l'} lA' NA').
+  
+  Lemma BoolIrrelevanceTyEq B : [Γ ||-<lA> A ≅ B | RA]< wl > -> [Γ ||-<lA'> A' ≅ B | RA']< wl >.
+  Proof.
+    intros []; now econstructor.
+  Qed.
+
+  Lemma BoolIrrelevanceTm :
+    (forall t, [Γ ||-<lA> t : A | RA]< wl > -> [Γ ||-<lA'> t : A' | RA']< wl >).
+  Proof.
+    intros t Ht. induction Ht. econstructor. exact red. assumption.
+    induction prop ; now econstructor.
+  Qed.
+   
+  Lemma BoolIrrelevanceTmEq :
+    (forall t u, [Γ ||-<lA> t ≅ u : A | RA]< wl > -> [Γ ||-<lA'> t ≅ u : A' | RA']< wl >).
+  Proof.
+    intros t u Htu ; induction Htu.
+    econstructor ; [ exact redL | exact redR | ..] ; try assumption.
+    induction prop ; now econstructor.
+  Qed.
+End BoolIrrelevant.
+
+Lemma BoolIrrelevanceLRPack@{i j k l i' j' k' l' v}
+  {wl Γ lA lA' A A'} (NA : [Γ ||-Bool A]< wl >) (NA' : [Γ ||-Bool A']< wl >)
+  (RA := LRBool_@{i j k l} lA NA) (RA' := LRBool_@{i' j' k' l'} lA' NA') :
+  equivLRPack@{k k' v} RA RA'.
+Proof.
+  constructor.
+  - split; apply BoolIrrelevanceTyEq.
+  - split; apply BoolIrrelevanceTm.
+  - split; apply BoolIrrelevanceTmEq.
+Qed.
+
+
+
 Section EmptyIrrelevant.
   Universe i j k l i' j' k' l'.
 
-  Context {Γ lA lA' A A'} (NA : [Γ ||-Empty A]) (NA' : [Γ ||-Empty A'])
+  Context {wl Γ lA lA' A A'} (NA : [Γ ||-Empty A]< wl >) (NA' : [Γ ||-Empty A']< wl >)
     (RA := LREmpty_@{i j k l} lA NA) (RA' := LREmpty_@{i' j' k' l'} lA' NA').
   
-  Lemma EmptyIrrelevanceTyEq B : [Γ ||-<lA> A ≅ B | RA] -> [Γ ||-<lA'> A' ≅ B | RA'].
+  Lemma EmptyIrrelevanceTyEq B : [Γ ||-<lA> A ≅ B | RA]< wl > -> [Γ ||-<lA'> A' ≅ B | RA']< wl >.
   Proof.
     intros []; now econstructor.
   Qed.
 
   Lemma EmptyIrrelevanceTm :
-    (forall t, [Γ ||-<lA> t : A | RA] -> [Γ ||-<lA'> t : A' | RA']).
+    (forall t, [Γ ||-<lA> t : A | RA]< wl > -> [Γ ||-<lA'> t : A' | RA']< wl >).
   Proof.
     intros t Ht. induction Ht; now econstructor.
   Qed.
    
   Lemma EmptyIrrelevanceTmEq :
-    (forall t u, [Γ ||-<lA> t ≅ u : A | RA] -> [Γ ||-<lA'> t ≅ u : A' | RA']).
+    (forall t u, [Γ ||-<lA> t ≅ u : A | RA]< wl > -> [Γ ||-<lA'> t ≅ u : A' | RA']< wl >).
   Proof.
     intros t u Htu. induction Htu. now econstructor.
   Qed.
 End EmptyIrrelevant.
 
 Lemma EmptyIrrelevanceLRPack@{i j k l i' j' k' l' v}
-  {Γ lA lA' A A'} (NA : [Γ ||-Empty A]) (NA' : [Γ ||-Empty A'])
+  {wl Γ lA lA' A A'} (NA : [Γ ||-Empty A]< wl >) (NA' : [Γ ||-Empty A']< wl >)
   (RA := LREmpty_@{i j k l} lA NA) (RA' := LREmpty_@{i' j' k' l'} lA' NA') :
   equivLRPack@{k k' v} RA RA'.
 Proof.
@@ -263,32 +470,32 @@ Universe i j k l i' j' k' l'.
 Definition IHStatement lA lA' :=
   (forall l0 (ltA : l0 << lA) (ltA' : l0 << lA'),
       prod@{v v}
-        (forall Γ t, [ LogRelRec@{i j k} lA l0 ltA | Γ ||- t ] <≈> [ LogRelRec@{i' j' k'} lA' l0 ltA' | Γ ||- t ])
-        (forall Γ t
-           (lr1 : [ LogRelRec@{i j k} lA l0 ltA | Γ ||- t ])
-           (lr2 : [ LogRelRec@{i' j' k'} lA' l0 ltA' | Γ ||- t ])
+        (forall wl Γ t, [ LogRelRec@{i j k} lA l0 ltA | Γ ||- t ]< wl > <≈> [ LogRelRec@{i' j' k'} lA' l0 ltA' | Γ ||- t ]< wl >)
+        (forall wl Γ t
+           (lr1 : [ LogRelRec@{i j k} lA l0 ltA | Γ ||- t ]< wl >)
+           (lr2 : [ LogRelRec@{i' j' k'} lA' l0 ltA' | Γ ||- t ]< wl >)
            u,
-            [ LogRelRec@{i j k} lA l0 ltA | Γ ||- t ≅ u | lr1 ] <≈>
-            [ LogRelRec@{i' j' k'} lA' l0 ltA' | Γ ||- t ≅ u | lr2 ])).
+            [ LogRelRec@{i j k} lA l0 ltA | Γ ||- t ≅ u | lr1 ]< wl > <≈>
+            [ LogRelRec@{i' j' k'} lA' l0 ltA' | Γ ||- t ≅ u | lr2 ]< wl >)).
 
 Lemma UnivIrrelevanceLRPack
-  {Γ lA lA' A A'}
+  {wl Γ lA lA' A A'}
   (IH : IHStatement lA lA')
-  (hU : [Γ ||-U<lA> A]) (hU' : [Γ ||-U<lA'> A'])
+  (hU : [Γ ||-U<lA> A]< wl >) (hU' : [Γ ||-U<lA'> A']< wl >)
   (RA := LRU_@{i j k l} hU) (RA' := LRU_@{i' j' k' l'} hU') :
   equivLRPack@{k k' v} RA RA'.
 Proof.
   revert IH; destruct hU as [_ []], hU' as [_ []]; intro IH; destruct (IH zero Oi Oi) as [IHty IHeq].
   constructor.
   + intros; cbn; split; intros []; now constructor.
-  + intros ?; destruct (IHty Γ t) as [tfwd tbwd]; split; intros [];
+  + intros ?; destruct (IHty wl Γ t) as [tfwd tbwd]; split; intros [];
       unshelve econstructor.
     7: now apply tfwd.
     11: now apply tbwd.
     all : tea.
   + cbn ; intros ? ?;
-    destruct (IHty Γ t) as [tfwd tbwd];
-    destruct (IHty Γ u) as [ufwd ubwd].
+    destruct (IHty wl Γ t) as [tfwd tbwd];
+    destruct (IHty wl Γ u) as [ufwd ubwd].
     split; intros [[] []]; cbn in *; unshelve econstructor.
     3: now apply tfwd.
     5: now apply tbwd.
@@ -296,8 +503,8 @@ Proof.
     8: now apply ubwd.
     (* all: apply todo. *)
     all: cbn.
-    6: now refine (fst (IHeq _ _ _ _ _) _).
-    7: now refine (snd (IHeq _ _ _ _ _) _).
+    6: now refine (fst (IHeq _ _ _ _ _ _) _).
+    7: now refine (snd (IHeq _ _ _ _ _ _) _).
     1-4: now econstructor.
     all: cbn; tea.
 Qed.
@@ -306,83 +513,96 @@ Qed.
 
 Lemma LRIrrelevantPreds {lA lA'}
   (IH : IHStatement lA lA')
-  (Γ : context) (A A' : term)
+  (wl : wfLCon) (Γ : context) (A A' : term)
   {eqTyA redTmA : term -> Type@{k}}
   {eqTyA' redTmA' : term -> Type@{k'}}
   {eqTmA : term -> term -> Type@{k}}
   {eqTmA' : term -> term -> Type@{k'}}
-  (lrA : LogRel@{i j k l} lA Γ A eqTyA redTmA eqTmA)
-  (lrA' : LogRel@{i' j' k' l'} lA' Γ A' eqTyA' redTmA' eqTmA')
-  (RA := Build_LRPack Γ A eqTyA redTmA eqTmA)
-  (RA' := Build_LRPack Γ A' eqTyA' redTmA' eqTmA') :
+  (lrA : LogRel@{i j k l} lA wl Γ A eqTyA redTmA eqTmA)
+  (lrA' : LogRel@{i' j' k' l'} lA' wl Γ A' eqTyA' redTmA' eqTmA')
+  (RA := Build_LRPack wl Γ A eqTyA redTmA eqTmA)
+  (RA' := Build_LRPack wl Γ A' eqTyA' redTmA' eqTmA') :
   eqTyA A' ->
   equivLRPack@{k k' v} RA RA'.
 Proof.
-  pose proof (fun Γ l0 ltA ltA' => fst (IH l0 ltA ltA') Γ) as IHty.
-  pose proof (fun Γ l0 ltA ltA' => snd (IH l0 ltA ltA') Γ) as IHeq.
+  pose proof (fun wl Γ l0 ltA ltA' => fst (IH l0 ltA ltA') wl Γ) as IHty.
+  pose proof (fun wl Γ l0 ltA ltA' => snd (IH l0 ltA ltA') wl Γ) as IHeq.
   intros he.
   set (s := ShapeViewConv lrA lrA' he).
-  induction lrA as [? ? h1 | ? ? neA | ? A ΠA HAad IHdom IHcod | ?? NA | ?? NA]
+  induction lrA as [? ? h1 | ? ? ? neA | ? ? A ΠA HAad IHdom IHcod | ?? NA | ?? NA | ?? NA]
     in RA, A', RA', eqTyA', eqTmA', redTmA', lrA', he, s |- *.
-  - destruct lrA' as [? ? h2 | | | |]; try solve [destruct s] ; clear s.
+  - destruct lrA' as [? ? h2 | | | | |]; try solve [destruct s] ; clear s.
     now apply UnivIrrelevanceLRPack.
-  - destruct lrA' as [|? A' neA'| | |] ; try solve [destruct s] ; clear s.
+  - destruct lrA' as [|? ? A' neA' | | | |] ; try solve [destruct s] ; clear s.
     exact (NeIrrelevanceLRPack lA lA' neA neA' he).
-  - destruct lrA' as [| | ? A' ΠA' HAad'| |] ; try solve [destruct s] ; clear s.
+  - cbn in *.
+    destruct lrA' as [| | ? ? A' ΠA' HAad' | | |] ; try solve [destruct s] ; clear s.
     pose (PA := PiRedTyPack.pack ΠA HAad).
     pose (PA' := PiRedTyPack.pack ΠA' HAad').
-    destruct he as [dom0 cod0 ?? domRed codRed], ΠA' as [dom1 cod1];
+    destruct he as [dom0 cod0 ??? domRed ? codRed], ΠA' as [dom1 cod1].
     assert (tProd dom0 cod0 = tProd dom1 cod1) as ePi
     by (eapply whredty_det ; gen_typing).
     inversion ePi ; subst ; clear ePi.
-    eapply (ΠIrrelevanceLRPack PA PA').
+    unshelve eapply (ΠIrrelevanceLRPack PA PA').
+    + exact domN.
+    + intros ; unshelve eapply codomN ; try assumption.
     + eassumption.
-    + intros; unshelve eapply IHdom.
-      1: eapply (LRAd.adequate (PiRedTyPack.domRed PA' _ _)).
-      eapply domRed.
+    + cbn in *.
+      intros; unshelve eapply IHdom.
+      1: now eapply (LRAd.adequate (PiRedTyPack.domRed PA' _ _ _ _)).
+      now eapply domRed.
     + intros; unshelve eapply IHcod.
-      1: eapply (LRAd.adequate (PiRedTyPack.codRed PA' _ _ _)).
-      eapply codRed.
-  - destruct lrA' as [| | ? A' ΠA' HAad'| |] ; try solve [destruct s] ; clear s.
+      1: eapply (LRAd.adequate (PiRedTyPack.codRed PA' _ _ _ _ _ _ _)).
+      now eapply codRed. 
+  - destruct lrA' as [| | ? A' ΠA' HAad'| | |] ; try solve [destruct s] ; clear s.
     apply (NatIrrelevanceLRPack (lA:=lA) (lA':=lA')).
-  - destruct lrA' as [| | ? A' ΠA' HAad'| |] ; try solve [destruct s] ; clear s.
+  - destruct lrA' as [| | ? A' ΠA' HAad'| | |] ; try solve [destruct s] ; clear s.
+    apply (BoolIrrelevanceLRPack (lA:=lA) (lA':=lA')).
+  - destruct lrA' as [| | ? A' ΠA' HAad'| | |] ; try solve [destruct s] ; clear s.
     apply (EmptyIrrelevanceLRPack (lA:=lA) (lA':=lA')).
 Qed.
 
 
 Lemma LRIrrelevantCumTy {lA}
   (IH : IHStatement lA lA)
-  (Γ : context) (A : term)
-  : [ LogRel@{i j k l} lA | Γ ||- A ] -> [ LogRel@{i' j' k' l'} lA | Γ ||- A ].
+  (wl : wfLCon) (Γ : context) (A : term)
+  : [ LogRel@{i j k l} lA | Γ ||- A ]< wl > -> [ LogRel@{i' j' k' l'} lA | Γ ||- A ]< wl >.
 Proof.
   intros [ [] lrA ] ; cbn in lrA.
-  induction lrA as [? ? [l1 lt1] | ? | ? A [] [] IHdom IHcod|?? NEA|?? NEA].
+  induction lrA as [? ? ? [l1 lt1] | ? | ? ? A [] [] IHdom IHcod|?? NEA|?? NEA |?? NEA].
   - eapply LRU_. econstructor ; tea.
   - eapply LRne_. exact neA.
   - cbn in *. eapply LRPi'. unshelve econstructor.
-    6: eassumption.
+    7: eassumption.
     4,5,6: tea.
+    + assumption.
     + exact IHdom.
-    + intros Δ a ρ tΔ ra. eapply IHcod.
-      destruct (LRIrrelevantPreds IH Δ (dom⟨ρ⟩) (dom⟨ρ⟩)
-                  (domAd Δ ρ tΔ) (IHdom Δ ρ tΔ : LRPackAdequate (LogRel@{i' j' k' l'} lA) (IHdom Δ ρ tΔ))
-                  (LRTyEqRefl (domAd Δ ρ tΔ))) as [_ irrTmRed _].
+    + intros Δ a wl' ρ τ Ninfl tΔ ra.
+      eapply codomN.
+      destruct (LRIrrelevantPreds IH wl' Δ (dom⟨ρ⟩) (dom⟨ρ⟩)
+                  (domAd Δ wl' ρ τ Ninfl tΔ)
+                  (IHdom Δ wl' ρ τ Ninfl tΔ : LRPackAdequate (LogRel@{i' j' k' l'} lA) (IHdom Δ wl' ρ τ Ninfl tΔ))
+                  (LRTyEqRefl (domAd Δ wl' ρ τ Ninfl tΔ))) as [_ irrTmRed _].
       eapply (snd (irrTmRed a)). exact ra.
-    + cbn. intros Δ a b ρ tΔ ra rb rab.
-      destruct (LRIrrelevantPreds IH Δ (dom⟨ρ⟩) (dom⟨ρ⟩)
-                  (domAd Δ ρ tΔ) (IHdom Δ ρ tΔ : LRPackAdequate (LogRel@{i' j' k' l'} lA) (IHdom Δ ρ tΔ))
-                  (LRTyEqRefl (domAd Δ ρ tΔ))) as [_ irrTmRed irrTmEq].
-      destruct (LRIrrelevantPreds IH Δ (cod[a .: ρ >> tRel]) (cod[a .: ρ >> tRel])
-                  (codAd Δ a ρ tΔ (snd (irrTmRed a) ra))
-                  (IHcod Δ a ρ tΔ (snd (irrTmRed a) ra)
-                    : LRPackAdequate (LogRel@{i' j' k' l'} lA) (IHcod Δ a ρ tΔ (snd (irrTmRed a) ra)))
-                  (LRTyEqRefl (codAd Δ a ρ tΔ (snd (irrTmRed a) ra))))
+    + intros Δ a wl' ρ τ Ninfl tΔ ra.
+      now eapply IHcod.
+    + assumption.
+    + cbn. intros Δ a b wl' ρ τ Ninfl tΔ ra rb rab wl'' τ' Minfl.
+      destruct (LRIrrelevantPreds IH wl' Δ (dom⟨ρ⟩) (dom⟨ρ⟩)
+                  (domAd  Δ wl' ρ τ Ninfl tΔ) (IHdom  Δ wl' ρ τ Ninfl tΔ : LRPackAdequate (LogRel@{i' j' k' l'} lA) (IHdom  Δ wl' ρ τ Ninfl tΔ))
+                  (LRTyEqRefl (domAd  Δ wl' ρ τ Ninfl tΔ))) as [_ irrTmRed irrTmEq].
+      destruct (LRIrrelevantPreds IH wl'' Δ (cod[a .: ρ >> tRel]) (cod[a .: ρ >> tRel])
+                  (codAd Δ a wl' ρ τ Ninfl tΔ (snd (irrTmRed a) ra) wl'' τ' Minfl)
+                  (IHcod Δ wl' a ρ τ Ninfl tΔ (snd (irrTmRed a) ra) wl'' τ' Minfl 
+                    : LRPackAdequate (LogRel@{i' j' k' l'} lA) (IHcod Δ wl' a ρ τ Ninfl tΔ (snd (irrTmRed a) ra) wl'' τ' Minfl))
+                  (LRTyEqRefl (codAd Δ a wl' ρ τ Ninfl tΔ (snd (irrTmRed a) ra) wl'' τ' Minfl)))
         as [irrTyEq _ _].
       eapply (fst (irrTyEq (cod[b .: ρ >> tRel]))).
       eapply codExt.
       exact (snd (irrTmRed b) rb).
       exact (snd (irrTmEq a b) rab).
   - now eapply LRNat_.
+  - now eapply LRBool_.
   - now eapply LREmpty_.
 Qed.
 
@@ -400,11 +620,11 @@ Proof.
   intros l0 ltA ltA'.
   destruct ltA. destruct ltA'. cbn in *.
   split.
-  - intros Γ t. split.
+  - intros wl Γ t. split.
     + eapply (LRIrrelevantCumTy@{u i j k u i' j' k'} IrrRec0@{u i j k u i' j' k'}).
     + eapply (LRIrrelevantCumTy@{u i' j' k' u i j k} IrrRec0@{u i' j' k' u i j k}).
-  - intros Γ t lr1 lr2 u.
-    destruct (LRIrrelevantPreds@{u i j k u i' j' k'} IrrRec0@{u i j k u i' j' k'} Γ t t
+  - intros wl Γ t lr1 lr2 u.
+    destruct (LRIrrelevantPreds@{u i j k u i' j' k'} IrrRec0@{u i j k u i' j' k'} wl Γ t t
                 (lr1 : LRPackAdequate (LogRel@{u i j k} zero) lr1)
                 (lr2 : LRPackAdequate (LogRel@{u i' j' k'} zero) lr2)
                 (LRTyEqRefl_ lr1)) as [tyEq _ _].
@@ -412,205 +632,205 @@ Proof.
 Qed.
 
 Theorem LRIrrelevantCum@{i j k l i' j' k' l'}
-  (Γ : context) (A A' : term) {lA lA'}
+  (wl : wfLCon) (Γ : context) (A A' : term) {lA lA'}
   {eqTyA redTmA : term -> Type@{k}}
   {eqTyA' redTmA' : term -> Type@{k'}}
   {eqTmA : term -> term -> Type@{k}}
   {eqTmA' : term -> term -> Type@{k'}}
-  (lrA : LogRel@{i j k l} lA Γ A eqTyA redTmA eqTmA)
-  (lrA' : LogRel@{i' j' k' l'} lA' Γ A' eqTyA' redTmA' eqTmA') :
+  (lrA : LogRel@{i j k l} lA wl Γ A eqTyA redTmA eqTmA)
+  (lrA' : LogRel@{i' j' k' l'} lA' wl Γ A' eqTyA' redTmA' eqTmA') :
   eqTyA A' ->
   @and3@{v v v} (forall B, eqTyA B <≈> eqTyA' B)
     (forall t, redTmA t <≈> redTmA' t)
     (forall t u, eqTmA t u <≈> eqTmA' t u).
 Proof.
-  exact (LRIrrelevantPreds@{i j k l i' j' k' l'} IrrRec Γ A A' lrA lrA').
+  exact (LRIrrelevantPreds@{i j k l i' j' k' l'} IrrRec wl Γ A A' lrA lrA').
 Qed.
 
 Theorem LRCumulative@{i j k l i' j' k' l'} {lA}
-  {Γ : context} {A : term}
-  : [ LogRel@{i j k l} lA | Γ ||- A ] -> [ LogRel@{i' j' k' l'} lA | Γ ||- A ].
+  {wl : wfLCon} {Γ : context} {A : term}
+  : [ LogRel@{i j k l} lA | Γ ||- A ]< wl > -> [ LogRel@{i' j' k' l'} lA | Γ ||- A ]< wl >.
 Proof.
-  exact (LRIrrelevantCumTy@{i j k l i' j' k' l'} IrrRec Γ A).
+  exact (LRIrrelevantCumTy@{i j k l i' j' k' l'} IrrRec wl Γ A).
 Qed.
 
 Corollary LRCumulative' @{i j k l i' j' k' l'} {lA}
-  {Γ : context} {A A' : term}
-  : A = A' -> [ LogRel@{i j k l} lA | Γ ||- A ] -> [ LogRel@{i' j' k' l'} lA | Γ ||- A' ].
+  {wl : wfLCon} {Γ : context} {A A' : term}
+  : A = A' -> [ LogRel@{i j k l} lA | Γ ||- A ]< wl > -> [ LogRel@{i' j' k' l'} lA | Γ ||- A' ]< wl >.
 Proof.
   intros ->; apply LRCumulative.
 Qed.
 End LRIrrelevant.
 
 
-Corollary TyEqIrrelevantCum Γ A {lA eqTyA redTmA eqTmA lA' eqTyA' redTmA' eqTmA'}
-  (lrA : LogRel lA Γ A eqTyA redTmA eqTmA) (lrA' : LogRel lA' Γ A eqTyA' redTmA' eqTmA') :
+Corollary TyEqIrrelevantCum wl Γ A {lA eqTyA redTmA eqTmA lA' eqTyA' redTmA' eqTmA'}
+  (lrA : LogRel lA wl Γ A eqTyA redTmA eqTmA) (lrA' : LogRel lA' wl Γ A eqTyA' redTmA' eqTmA') :
   forall B, eqTyA B -> eqTyA' B.
 Proof.
-  apply (LRIrrelevantCum _ _ _ lrA lrA').
+  apply (LRIrrelevantCum _ _ _ _ lrA lrA').
   now eapply LRTyEqRefl.
 Qed.
 
-Corollary LRTyEqIrrelevantCum@{i j k l i' j' k' l'} lA lA' Γ A
-  (lrA : [LogRel@{i j k l} lA | Γ ||- A]) (lrA' : [LogRel@{i' j' k' l'} lA' | Γ ||- A]) :
-  forall B, [Γ ||-< lA > A ≅ B | lrA] -> [Γ ||-< lA' > A ≅ B | lrA'].
+Corollary LRTyEqIrrelevantCum@{i j k l i' j' k' l'} lA lA' wl Γ A
+  (lrA : [LogRel@{i j k l} lA | Γ ||- A]< wl >) (lrA' : [LogRel@{i' j' k' l'} lA' | Γ ||- A]< wl >) :
+  forall B, [Γ ||-< lA > A ≅ B | lrA]< wl > -> [Γ ||-< lA' > A ≅ B | lrA']< wl >.
 Proof.
   destruct lrA, lrA'.
   cbn in *.
   now eapply TyEqIrrelevantCum.
 Qed.
 
-Corollary LRTyEqIrrelevantCum'@{i j k l i' j' k' l'} lA lA' Γ A A' (e : A = A')
-  (lrA : [LogRel@{i j k l} lA | Γ ||- A]) (lrA' : [LogRel@{i' j' k' l'} lA' | Γ ||- A']) :
-  forall B, [Γ ||-< lA > A ≅ B | lrA] -> [Γ ||-< lA' > A' ≅ B | lrA'].
+Corollary LRTyEqIrrelevantCum'@{i j k l i' j' k' l'} lA lA' wl Γ A A' (e : A = A')
+  (lrA : [LogRel@{i j k l} lA | Γ ||- A]< wl >) (lrA' : [LogRel@{i' j' k' l'} lA' | Γ ||- A']< wl >) :
+  forall B, [Γ ||-< lA > A ≅ B | lrA]< wl > -> [Γ ||-< lA' > A' ≅ B | lrA']< wl >.
 Proof.
   revert lrA'; rewrite <- e; now apply LRTyEqIrrelevantCum.
 Qed.
 
-Corollary LRTyEqIrrelevant'@{i j k l} lA lA' Γ A A' (e : A = A')
-  (lrA : [LogRel@{i j k l} lA | Γ ||- A]) (lrA' : [LogRel@{i j k l} lA' | Γ ||- A']) :
-  forall B, [Γ ||-< lA > A ≅ B | lrA] -> [Γ ||-< lA' > A' ≅ B | lrA'].
+Corollary LRTyEqIrrelevant'@{i j k l} lA lA' wl Γ A A' (e : A = A')
+  (lrA : [LogRel@{i j k l} lA | Γ ||- A]< wl >) (lrA' : [LogRel@{i j k l} lA' | Γ ||- A']< wl >) :
+  forall B, [Γ ||-< lA > A ≅ B | lrA]< wl > -> [Γ ||-< lA' > A' ≅ B | lrA']< wl >.
 Proof.
   revert lrA'; rewrite <- e; now apply LRTyEqIrrelevantCum.
 Qed.
 
-Corollary RedTmIrrelevantCum Γ A {lA eqTyA redTmA eqTmA lA' eqTyA' redTmA' eqTmA'}
-  (lrA : LogRel lA Γ A eqTyA redTmA eqTmA) (lrA' : LogRel lA' Γ A eqTyA' redTmA' eqTmA') :
+Corollary RedTmIrrelevantCum wl Γ A {lA eqTyA redTmA eqTmA lA' eqTyA' redTmA' eqTmA'}
+  (lrA : LogRel lA wl Γ A eqTyA redTmA eqTmA) (lrA' : LogRel lA' wl Γ A eqTyA' redTmA' eqTmA') :
   forall t, redTmA t -> redTmA' t.
 Proof.
-  apply (LRIrrelevantCum _ _ _ lrA lrA').
+  apply (LRIrrelevantCum _ _ _ _ lrA lrA').
   now eapply LRTyEqRefl.
 Qed.
 
-Corollary LRTmRedIrrelevantCum@{i j k l i' j' k' l'} lA lA' Γ A
-  (lrA : [LogRel@{i j k l} lA | Γ ||- A]) (lrA' : [LogRel@{i' j' k' l'} lA' | Γ ||- A]) :
-  forall t, [Γ ||-< lA > t : A | lrA] -> [Γ ||-< lA' > t : A | lrA'].
+Corollary LRTmRedIrrelevantCum@{i j k l i' j' k' l'} lA lA' wl Γ A
+  (lrA : [LogRel@{i j k l} lA | Γ ||- A]< wl >) (lrA' : [LogRel@{i' j' k' l'} lA' | Γ ||- A]< wl >) :
+  forall t, [Γ ||-< lA > t : A | lrA]< wl > -> [Γ ||-< lA' > t : A | lrA']< wl >.
 Proof.
   destruct lrA, lrA'.
   cbn in *.
   now eapply RedTmIrrelevantCum.
 Qed.
 
-Corollary LRTmRedIrrelevantCum'@{i j k l i' j' k' l'} lA lA' Γ A A' (e : A = A')
-  (lrA : [LogRel@{i j k l} lA | Γ ||- A]) (lrA' : [LogRel@{i' j' k' l'} lA' | Γ ||- A']) :
-  forall t, [Γ ||-< lA > t : A | lrA] -> [Γ ||-< lA' > t : A' | lrA'].
+Corollary LRTmRedIrrelevantCum'@{i j k l i' j' k' l'} lA lA' wl Γ A A' (e : A = A')
+  (lrA : [LogRel@{i j k l} lA | Γ ||- A]< wl >) (lrA' : [LogRel@{i' j' k' l'} lA' | Γ ||- A']< wl >) :
+  forall t, [Γ ||-< lA > t : A | lrA]< wl > -> [Γ ||-< lA' > t : A' | lrA']< wl >.
 Proof.
   revert lrA'; rewrite <- e; now apply LRTmRedIrrelevantCum.
 Qed.
 
-Corollary LRTmRedIrrelevant'@{i j k l} lA lA' Γ A A' (e : A = A')
-  (lrA : [LogRel@{i j k l} lA | Γ ||- A]) (lrA' : [LogRel@{i j k l} lA' | Γ ||- A']) :
-  forall t, [Γ ||-< lA > t : A | lrA] -> [Γ ||-< lA' > t : A' | lrA'].
+Corollary LRTmRedIrrelevant'@{i j k l} lA lA' wl Γ A A' (e : A = A')
+  (lrA : [LogRel@{i j k l} lA | Γ ||- A]< wl >) (lrA' : [LogRel@{i j k l} lA' | Γ ||- A']< wl >) :
+  forall t, [Γ ||-< lA > t : A | lrA]< wl > -> [Γ ||-< lA' > t : A' | lrA']< wl >.
 Proof.
   revert lrA'; rewrite <- e; now apply LRTmRedIrrelevantCum.
 Qed.
 
 
-Corollary TmEqIrrelevantCum Γ A {lA eqTyA redTmA eqTmA lA' eqTyA' redTmA' eqTmA'}
-  (lrA : LogRel lA Γ A eqTyA redTmA eqTmA) (lrA' : LogRel lA' Γ A eqTyA' redTmA' eqTmA') :
+Corollary TmEqIrrelevantCum wl Γ A {lA eqTyA redTmA eqTmA lA' eqTyA' redTmA' eqTmA'}
+  (lrA : LogRel lA wl Γ A eqTyA redTmA eqTmA) (lrA' : LogRel lA' wl Γ A eqTyA' redTmA' eqTmA') :
   forall t u, eqTmA t u -> eqTmA' t u.
 Proof.
-  apply (LRIrrelevantCum _ _ _ lrA lrA').
+  apply (LRIrrelevantCum _ _ _ _ lrA lrA').
   now eapply LRTyEqRefl.
 Qed.
 
-Corollary LRTmEqIrrelevantCum@{i j k l i' j' k' l'} lA lA' Γ A
-  (lrA : [LogRel@{i j k l} lA | Γ ||- A]) (lrA' : [LogRel@{i' j' k' l'} lA' | Γ ||- A]) :
-  forall t u, [Γ ||-< lA > t ≅ u : A | lrA] -> [Γ ||-< lA' > t ≅ u : A | lrA'].
+Corollary LRTmEqIrrelevantCum@{i j k l i' j' k' l'} lA lA' wl Γ A
+  (lrA : [LogRel@{i j k l} lA | Γ ||- A]< wl >) (lrA' : [LogRel@{i' j' k' l'} lA' | Γ ||- A]< wl >) :
+  forall t u, [Γ ||-< lA > t ≅ u : A | lrA]< wl > -> [Γ ||-< lA' > t ≅ u : A | lrA']< wl >.
 Proof.
   destruct lrA, lrA'.
   cbn in *.
   now eapply TmEqIrrelevantCum.
 Qed.
 
-Corollary LRTmEqIrrelevantCum'@{i j k l i' j' k' l'} lA lA' Γ A A' (e : A = A')
-  (lrA : [LogRel@{i j k l} lA | Γ ||- A]) (lrA' : [LogRel@{i' j' k' l'} lA' | Γ ||- A']) :
-  forall t u, [Γ ||-< lA > t ≅ u : A | lrA] -> [Γ ||-< lA' > t ≅ u : A' | lrA'].
+Corollary LRTmEqIrrelevantCum'@{i j k l i' j' k' l'} lA lA' wl Γ A A' (e : A = A')
+  (lrA : [LogRel@{i j k l} lA | Γ ||- A]< wl >) (lrA' : [LogRel@{i' j' k' l'} lA' | Γ ||- A']< wl >) :
+  forall t u, [Γ ||-< lA > t ≅ u : A | lrA]< wl > -> [Γ ||-< lA' > t ≅ u : A' | lrA']< wl >.
 Proof.
   revert lrA'; rewrite <- e; now apply LRTmEqIrrelevantCum.
 Qed.
 
-Corollary LRTmEqIrrelevant'@{i j k l} lA lA' Γ A A' (e : A = A')
-  (lrA : [LogRel@{i j k l} lA | Γ ||- A]) (lrA' : [LogRel@{i j k l} lA' | Γ ||- A']) :
-  forall t u, [Γ ||-< lA > t ≅ u : A | lrA] -> [Γ ||-< lA' > t ≅ u : A' | lrA'].
+Corollary LRTmEqIrrelevant'@{i j k l} lA lA' wl Γ A A' (e : A = A')
+  (lrA : [LogRel@{i j k l} lA | Γ ||- A]< wl >) (lrA' : [LogRel@{i j k l} lA' | Γ ||- A']< wl >) :
+  forall t u, [Γ ||-< lA > t ≅ u : A | lrA]< wl > -> [Γ ||-< lA' > t ≅ u : A' | lrA']< wl >.
 Proof.
   revert lrA'; rewrite <- e; now apply LRTmEqIrrelevantCum.
 Qed.
 
 
 
-Corollary TyEqSym Γ A A' {lA eqTyA redTmA eqTmA lA' eqTyA' redTmA' eqTmA'}
-  (lrA : LogRel lA Γ A eqTyA redTmA eqTmA) (lrA' : LogRel lA' Γ A' eqTyA' redTmA' eqTmA') :
+Corollary TyEqSym wl Γ A A' {lA eqTyA redTmA eqTmA lA' eqTyA' redTmA' eqTmA'}
+  (lrA : LogRel lA wl Γ A eqTyA redTmA eqTmA) (lrA' : LogRel lA' wl Γ A' eqTyA' redTmA' eqTmA') :
   eqTyA A' -> eqTyA' A.
 Proof.
   intros.
-  apply (LRIrrelevantCum _ _ _ lrA lrA').
+  apply (LRIrrelevantCum _ _ _ _ lrA lrA').
   1: eauto.
   now eapply LRTyEqRefl.
 Qed.
 
-Corollary LRTyEqSym lA lA' Γ A A' (lrA : [Γ ||-< lA > A]) (lrA' : [Γ ||-< lA'> A']) :
-  [Γ ||-< lA > A ≅ A' | lrA] -> [Γ ||-< lA' > A' ≅ A | lrA'].
+Corollary LRTyEqSym lA lA' wl Γ A A' (lrA : [Γ ||-< lA > A]< wl >) (lrA' : [Γ ||-< lA'> A']< wl >) :
+  [Γ ||-< lA > A ≅ A' | lrA]< wl > -> [Γ ||-< lA' > A' ≅ A | lrA']< wl >.
 Proof.
   destruct lrA, lrA'.
   cbn in *.
   now eapply TyEqSym.
 Qed.
 
-Corollary RedTmConv Γ A A' {lA eqTyA redTmA eqTmA lA' eqTyA' redTmA' eqTmA'}
-  (lrA : LogRel lA Γ A eqTyA redTmA eqTmA) (lrA' : LogRel lA' Γ A' eqTyA' redTmA' eqTmA') :
+Corollary RedTmConv wl Γ A A' {lA eqTyA redTmA eqTmA lA' eqTyA' redTmA' eqTmA'}
+  (lrA : LogRel lA wl Γ A eqTyA redTmA eqTmA) (lrA' : LogRel lA' wl Γ A' eqTyA' redTmA' eqTmA') :
   eqTyA A' ->
   forall t, redTmA t -> redTmA' t.
 Proof.
-  apply (LRIrrelevantCum _ _ _ lrA lrA').
+  apply (LRIrrelevantCum _ _ _ _ lrA lrA').
 Qed.
 
-Corollary LRTmRedConv lA lA' Γ A A' (lrA : [Γ ||-< lA > A]) (lrA' : [Γ ||-< lA'> A' ]) :
-  [Γ ||-< lA > A ≅ A' | lrA ] ->
-  forall t, [Γ ||-< lA > t : A | lrA] -> [Γ ||-< lA' > t : A' | lrA'].
+Corollary LRTmRedConv lA lA' wl Γ A A' (lrA : [Γ ||-< lA > A]< wl >) (lrA' : [Γ ||-< lA'> A' ]< wl >) :
+  [Γ ||-< lA > A ≅ A' | lrA ]< wl > ->
+  forall t, [Γ ||-< lA > t : A | lrA]< wl > -> [Γ ||-< lA' > t : A' | lrA']< wl >.
 Proof.
   destruct lrA, lrA'.
   cbn in *.
   now eapply RedTmConv.
 Qed.
 
-Corollary TmEqRedConv Γ A A' {lA eqTyA redTmA eqTmA lA' eqTyA' redTmA' eqTmA'}
-  (lrA : LogRel lA Γ A eqTyA redTmA eqTmA) (lrA' : LogRel lA' Γ A' eqTyA' redTmA' eqTmA') :
+Corollary TmEqRedConv wl Γ A A' {lA eqTyA redTmA eqTmA lA' eqTyA' redTmA' eqTmA'}
+  (lrA : LogRel lA wl Γ A eqTyA redTmA eqTmA) (lrA' : LogRel lA' wl Γ A' eqTyA' redTmA' eqTmA') :
   eqTyA A' ->
   forall t u, eqTmA t u -> eqTmA' t u.
 Proof.
-  apply (LRIrrelevantCum _ _ _ lrA lrA').
+  apply (LRIrrelevantCum _ _ _ _ lrA lrA').
 Qed.
 
-Corollary LRTmEqRedConv lA lA' Γ A A' (lrA : [Γ ||-< lA > A]) (lrA' : [Γ ||-< lA'> A']) :
-  [Γ ||-< lA > A ≅ A' | lrA ] ->
-  forall t u, [Γ ||-< lA > t ≅ u : A | lrA] -> [Γ ||-< lA' > t ≅ u : A' | lrA'].
+Corollary LRTmEqRedConv lA lA' wl Γ A A' (lrA : [Γ ||-< lA > A]< wl >) (lrA' : [Γ ||-< lA'> A']< wl >) :
+  [Γ ||-< lA > A ≅ A' | lrA ]< wl > ->
+  forall t u, [Γ ||-< lA > t ≅ u : A | lrA]< wl > -> [Γ ||-< lA' > t ≅ u : A' | lrA']< wl >.
 Proof.
   destruct lrA, lrA'.
   cbn in *.
   now eapply TmEqRedConv.
 Qed.
 
-Corollary LRTmTmEqIrrelevant' lA lA' Γ A A' (e : A = A')
-  (lrA : [Γ ||-< lA > A]) (lrA' : [Γ ||-< lA'> A']) :
+Corollary LRTmTmEqIrrelevant' lA lA' wl Γ A A' (e : A = A')
+  (lrA : [Γ ||-< lA > A]< wl >) (lrA' : [Γ ||-< lA'> A']< wl >) :
   forall t u, 
-  [Γ ||-<lA> t : A | lrA] × [Γ ||-< lA > t ≅ u : A | lrA] -> 
-  [Γ ||-<lA'> t : A' | lrA'] × [Γ ||-< lA' > t ≅ u : A' | lrA'].
+  [Γ ||-<lA> t : A | lrA]< wl > × [Γ ||-< lA > t ≅ u : A | lrA]< wl > -> 
+  [Γ ||-<lA'> t : A' | lrA']< wl > × [Γ ||-< lA' > t ≅ u : A' | lrA']< wl >.
 Proof.
   intros ?? []; split; [eapply LRTmRedIrrelevant'| eapply LRTmEqIrrelevant']; tea.
 Qed.
 
 Set Printing Primitive Projection Parameters.
 
-Lemma NeNfEqSym {Γ k k' A} : [Γ ||-NeNf k ≅ k' : A] -> [Γ ||-NeNf k' ≅ k : A].
+Lemma NeNfEqSym {wl Γ k k' A} : [Γ ||-NeNf k ≅ k' : A]< wl > -> [Γ ||-NeNf k' ≅ k : A]< wl >.
 Proof.
   intros []; constructor; tea; now symmetry.
 Qed.
 
-Lemma LRTmEqSym@{h i j k l} lA Γ A (lrA : [LogRel@{i j k l} lA | Γ ||- A]) : forall t u,
-  [Γ ||-<lA> t ≅ u : A |lrA] -> [Γ ||-<lA> u ≅ t : A |lrA].
+Lemma LRTmEqSym@{h i j k l} lA wl Γ A (lrA : [LogRel@{i j k l} lA | Γ ||- A]< wl >) : forall t u,
+  [Γ ||-<lA> t ≅ u : A |lrA]< wl > -> [Γ ||-<lA> u ≅ t : A |lrA]< wl >.
 Proof.
-  pattern lA, Γ, A, lrA. apply LR_rect_TyUr; clear lA Γ A lrA.
+  pattern lA, wl, Γ, A, lrA. apply LR_rect_TyUr; clear lA Γ A lrA.
   - intros * []. unshelve econstructor; try eassumption.
     1: symmetry; eassumption.
     (* Need an additional universe level h < i *)
@@ -622,17 +842,27 @@ Proof.
     symmetry; eassumption.
   - intros * ihdom ihcod * []. unshelve econstructor.
     1,2: eassumption.
+    assumption.
+    assumption.
     1: symmetry; eassumption.
-    intros. apply ihcod. eapply eqApp.
-  - intros ??? NA.
+    intros. apply ihcod. now eapply eqApp.
+  - intros ???? NA.
     set (G := _); enough (h : G × (forall t u, NatPropEq NA t u -> NatPropEq NA u t)) by apply h.
     subst G; apply NatRedEqInduction.
     1-3: now econstructor.
-    intros; constructor; now eapply NeNfEqSym.
-  - intros ??? NA.
-    intros t u [? ? ? ? ? ? ? prop]. destruct prop. econstructor; eauto.
-    2: econstructor; now eapply NeNfEqSym.
-    symmetry; eassumption.
+    intros. constructor; now eapply NeNfEqSym.
+  - intros ???? NA.
+    intros t u [? ? ? ? ? ? ? prop]. induction prop.
+    + econstructor; eauto ; now econstructor.
+    + econstructor; eauto ; now econstructor.
+    + econstructor ; eauto.
+      * easy.
+      * constructor. now eapply NeNfEqSym.
+  - intros ???? NA.
+    intros t u [? ? ? ? ? ? ? prop]. induction prop.
+    econstructor ; eauto.
+    * easy.
+    * constructor. now eapply NeNfEqSym.
 Qed.
 
 End Irrelevances.
@@ -642,13 +872,13 @@ End Irrelevances.
 
 Ltac irrelevanceCum0 :=
   lazymatch goal with
-  | [|- [_ ||-<_> _]] => (now eapply LRCumulative) + eapply LRCumulative'
-  | [|- [_ | _ ||- _ ≅ _ ] ] => eapply LRTyEqIrrelevantCum'
-  | [|- [_ ||-<_> _ ≅ _ | _ ] ] => eapply LRTyEqIrrelevantCum'
-  | [|- [_ | _ ||- _ : _ ] ] => eapply LRTmRedIrrelevantCum'
-  | [|- [_ ||-<_> _ : _ | _ ] ] => eapply LRTmRedIrrelevantCum'
-  | [|- [_ | _ ||- _ ≅ _ : _ ] ] => eapply LRTmEqIrrelevantCum'
-  | [|- [_ ||-<_> _ ≅ _ : _ | _ ] ] => eapply LRTmEqIrrelevantCum'
+  | [|- [_ ||-<_> _]< _ >] => (now eapply LRCumulative) + eapply LRCumulative'
+  | [|- [_ | _ ||- _ ≅ _ ]< _ > ] => eapply LRTyEqIrrelevantCum'
+  | [|- [_ ||-<_> _ ≅ _ | _ ]< _ > ] => eapply LRTyEqIrrelevantCum'
+  | [|- [_ | _ ||- _ : _ ]< _ > ] => eapply LRTmRedIrrelevantCum'
+  | [|- [_ ||-<_> _ : _ | _ ]< _ > ] => eapply LRTmRedIrrelevantCum'
+  | [|- [_ | _ ||- _ ≅ _ : _ ]< _ > ] => eapply LRTmEqIrrelevantCum'
+  | [|- [_ ||-<_> _ ≅ _ : _ | _ ]< _ > ] => eapply LRTmEqIrrelevantCum'
   end.
 
 Ltac irrelevanceCum := irrelevanceCum0 ; [|eassumption] ; try first [reflexivity| now bsimpl].
@@ -657,13 +887,13 @@ Ltac irrelevanceCumRefl := irrelevanceCum0 ; [reflexivity|].
 
 Ltac irrelevance0 :=
   lazymatch goal with
-  | [|- [_ | _ ||- _ ≅ _ ] ] => eapply LRTyEqIrrelevant'
-  | [|- [_ ||-<_> _ ≅ _ | _ ] ] => eapply LRTyEqIrrelevant'
-  | [|- [_ | _ ||- _ : _ ] ] => eapply LRTmRedIrrelevant'
-  | [|- [_ ||-<_> _ : _ | _ ] ] => eapply LRTmRedIrrelevant'
-  | [|- [_ | _ ||- _ ≅ _ : _ ] ] => eapply LRTmEqIrrelevant'
-  | [|- [_ ||-<_> _ ≅ _ : _ | _ ] ] => eapply LRTmEqIrrelevant'
-  | [|- [_ ||-<_> _ : _ | _] × [_ ||-<_> _≅ _ : _ | _]] => eapply LRTmTmEqIrrelevant'
+  | [|- [_ | _ ||- _ ≅ _ ]< _ > ] => eapply LRTyEqIrrelevant'
+  | [|- [_ ||-<_> _ ≅ _ | _ ]< _ > ] => eapply LRTyEqIrrelevant'
+  | [|- [_ | _ ||- _ : _ ]< _ > ] => eapply LRTmRedIrrelevant'
+  | [|- [_ ||-<_> _ : _ | _ ]< _ > ] => eapply LRTmRedIrrelevant'
+  | [|- [_ | _ ||- _ ≅ _ : _ ]< _ > ] => eapply LRTmEqIrrelevant'
+  | [|- [_ ||-<_> _ ≅ _ : _ | _ ]< _ > ] => eapply LRTmEqIrrelevant'
+  | [|- [_ ||-<_> _ : _ | _]< _ > × [_ ||-<_> _≅ _ : _ | _]< _ >] => eapply LRTmTmEqIrrelevant'
   end.
 
 Ltac irrelevance := irrelevance0 ; [|eassumption] ; try first [reflexivity| now bsimpl].
