theories/LogicalRelation/Escape.v
@@ -1,7 +1,7 @@
 (** * LogRel.LogicalRelation.Escape: the logical relation implies conversion/typing. *)
 From Coq Require Import CRelationClasses.
 From LogRel.AutoSubst Require Import core unscoped Ast Extra.
-From LogRel Require Import Utils BasicAst Notations Context NormalForms GenericTyping LogicalRelation DeclarativeInstance.
+From LogRel Require Import Utils BasicAst Notations LContexts Context NormalForms GenericTyping LogicalRelation DeclarativeInstance.
 From LogRel.LogicalRelation Require Import Induction.
 
 Set Universe Polymorphism.
@@ -9,84 +9,90 @@ Set Universe Polymorphism.
 Section Escapes.
   Context `{GenericTypingProperties}.
 
-  Lemma escape {l Γ A} :
-      [Γ ||-< l > A ] ->
-      [Γ |- A].
+  Lemma escape {l wl Γ A} :
+      [Γ ||-< l > A ]< wl > ->
+      [Γ |- A]< wl >.
   Proof.
     intros lr.
-    pattern l, Γ, A, lr.
+    pattern l, wl,  Γ, A, lr.
     eapply LR_rect_TyUr.
     - intros * [].
       now gen_typing.
     - intros ? * [].
       now gen_typing.
-    - intros ??? [] **; cbn in *.
+    - intros ???? [] **; cbn in *.
       now gen_typing.
-    - intros ??? []; gen_typing.
-    - intros ??? []; gen_typing.
+    - intros ???? []; gen_typing.
+    - intros ???? []; gen_typing.
+    - intros ???? []; gen_typing.
   Qed.
 
-  Lemma escapeEq {l Γ A B} (lr : [Γ ||-< l > A]) :
-      [ Γ ||-< l > A ≅ B | lr ] ->
-      [Γ |- A ≅ B].
+  Lemma escapeEq {l wl Γ A B} (lr : [Γ ||-< l > A]< wl >) :
+      [ Γ ||-< l > A ≅ B | lr ]< wl > ->
+      [Γ |- A ≅ B]< wl >.
   Proof.
-    pattern l, Γ, A, lr ; eapply LR_rect_TyUr.
-    + intros ??? [] []. 
+    pattern l, wl, Γ, A, lr ; eapply LR_rect_TyUr.
+    + intros ???? [] []. 
       gen_typing.
-    + intros ??? [] [].
+    + intros ???? [] [].
       cbn in *.
       eapply convty_exp.
       all: gen_typing.
-    + intros ??? [] * ? ? [] ; cbn in *.
+    + intros ???? [] * ? ? [] ; cbn in *.
       gen_typing.
-    + intros ??? [] []; gen_typing.
-    + intros ??? [] []; gen_typing.
+    + intros ???? [] []; gen_typing.
+    + intros ???? [] []; gen_typing.
+    + intros ???? [] []; gen_typing.
   Qed.
 
-  Definition escapeTerm {l Γ t A} (lr : [Γ ||-< l > A ]) :
-    [Γ ||-< l > t : A | lr ] ->
-    [Γ |- t : A].
+  Definition escapeTerm {l wl Γ t A} (lr : [Γ ||-< l > A ]< wl >) :
+    [Γ ||-< l > t : A | lr ]< wl > ->
+    [Γ |- t : A]< wl >.
   Proof.
-    pattern l, Γ, A, lr ; eapply LR_rect_TyUr.
-    - intros ??? [] [] ; cbn in *.
+    pattern l, wl, Γ, A, lr ; eapply LR_rect_TyUr.
+    - intros ???? [] [] ; cbn in *.
       gen_typing.
-    - intros ??? [] [] ; cbn in *.
+    - intros ???? [] [] ; cbn in *.
       gen_typing.
-    - intros ??? [] * ?? [] ; cbn in *.
+    - intros ???? [] * ?? [] ; cbn in *.
       gen_typing.
-    - intros ??? [] []; gen_typing.
-    - intros ??? [] []; gen_typing.
+    - intros ???? [] []; gen_typing.
+    - intros ???? [] []; gen_typing.
+    - intros ???? [] []; gen_typing.
   Qed.
 
-  Definition escapeEqTerm {l Γ t u A} (lr : [Γ ||-< l > A ]) :
-    [Γ ||-< l > t ≅ u : A | lr ] ->
-    [Γ |- t ≅ u : A].
+  Definition escapeEqTerm {l wl Γ t u A} (lr : [Γ ||-< l > A ]< wl >) :
+    [Γ ||-< l > t ≅ u : A | lr ]< wl > ->
+    [Γ |- t ≅ u : A]< wl >.
   Proof.
-    pattern l, Γ, A, lr ; eapply LR_rect_TyUr.
-    - intros ??? [] [[] []] ; cbn in *.
+    pattern l, wl, Γ, A, lr ; eapply LR_rect_TyUr.
+    - intros ???? [] [[] []] ; cbn in *.
       eapply convtm_exp ; tea.
       all: gen_typing.
-    - intros ??? [] [] ; cbn in *.
+    - intros ???? [] [] ; cbn in *.
       eapply convtm_exp ; tea.
       all: gen_typing.
-    - intros ??? [] * ?? [[termL] [termR]] ; cbn in *.
+    - intros ???? [] * ?? [[termL] [termR]] ; cbn in *.
       eapply convtm_exp ; tea.
       all: gen_typing.
-    - intros ??? [] []; cbn in *.
+    - intros ???? [] []; cbn in *.
       eapply convtm_exp; tea; gen_typing.
-    - intros ??? [] []; cbn in *.
+    - intros ???? [] []; cbn in *.
+      eapply convtm_exp; tea; gen_typing.
+    - intros ???? [] []; cbn in *.
       eapply convtm_exp; tea; gen_typing.
   Qed.
 
-  Lemma escapeConv {l Γ A} (RA : [Γ ||-<l> A]) :
+  Lemma escapeConv {l wl Γ A} (RA : [Γ ||-<l> A]< wl >) :
     forall B,
-    [Γ ||-<l> A ≅ B | RA] ->
-    [Γ |- B].
+    [Γ ||-<l> A ≅ B | RA]< wl > ->
+    [Γ |- B]< wl >.
   Proof.
-    pattern l, Γ, A, RA; eapply LR_rect_TyUr; clear l Γ A RA.
+    pattern l, wl, Γ, A, RA; eapply LR_rect_TyUr; clear l Γ A RA.
     - intros * []; gen_typing.
     - intros * []; gen_typing.
     - intros * ihdom ihcod ? []; gen_typing.
+    - intros * []; gen_typing.
     - intros * []; gen_typing.
     - intros * []; gen_typing.
   Qed.
@@ -95,19 +101,19 @@ End Escapes.
 
 Ltac escape :=
   repeat lazymatch goal with
-  | [H : [_ ||-< _ > _] |- _] => 
+  | [H : [_ ||-< _ > _]< _ > |- _] => 
     let X := fresh "Esc" H in
     try pose proof (X := escape H) ;
     block H
-  | [H : [_ ||-<_> _ ≅ _ | ?RA ] |- _] =>
+  | [H : [_ ||-<_> _ ≅ _ | ?RA ]< _ > |- _] =>
     let X := fresh "Esc" H in
     try pose proof (X := escapeEq RA H) ;
     block H
-  | [H : [_ ||-<_> _ : _ | ?RA] |- _] =>
+  | [H : [_ ||-<_> _ : _ | ?RA]< _ > |- _] =>
     let X := fresh "R" H in
     try pose proof (X := escapeTerm RA H) ;
     block H
-  | [H : [_ ||-<_> _ ≅ _ : _ | ?RA] |- _] =>
+  | [H : [_ ||-<_> _ ≅ _ : _ | ?RA]< _ > |- _] =>
     let X := fresh "R" H in
     try pose proof (X := escapeEqTerm RA H) ;
     block H
